Proved DNS cache lemmas.

src/BinEncoders/Env/Examples/DnsOpt.v
@@ -1,5 +1,6 @@
 Require Import
         Coq.Strings.String
+        Coq.Arith.Mult
         Coq.Vectors.Vector.
 
 Require Import
@@ -7,6 +8,7 @@ Require Import
         Fiat.Common.SumType
         Fiat.Common.BoundedLookup
         Fiat.Common.ilist
+        Fiat.Common.DecideableEnsembles
         Fiat.Computation
         Fiat.QueryStructure.Specification.Representation.Notations
         Fiat.QueryStructure.Specification.Representation.Heading
@@ -29,26 +31,519 @@ Require Import
 Require Import
         Bedrock.Word.
 
-Import Vectors.VectorDef.VectorNotations.
-
 Section DnsPacket.
 
   Open Scope Tuple_scope.
 
-  Variable cache : Cache.
-  Variable cacheAddNat : CacheAdd cache nat.
-  Variable cacheAddDNPointer : CacheAdd cache (string * pointerT).
-  Variable cacheGetDNPointer : CacheGet cache string pointerT.
-  Variable cachePeekDNPointer : CachePeek cache pointerT.
-  Variable IndependentCaches :
+  Definition association_list K V := list (K * V).
+
+  Fixpoint association_list_find_first {K V}
+           {K_eq : Query_eq K}
+           (l : association_list K V)
+           (k : K) : option V :=
+    match l with
+    | (k', v) :: l' => if A_eq_dec k k' then Some v else association_list_find_first l' k
+    | _ => None
+    end.
+
+  Fixpoint association_list_find_all {K V}
+           {K_eq : Query_eq K}
+           (l : association_list K V)
+           (k : K) : list V :=
+    match l with
+    | (k', v) :: l' => if A_eq_dec k k' then v :: association_list_find_all l' k
+                       else association_list_find_all l' k
+    | _ => nil
+    end.
+
+  Fixpoint association_list_add {K V}
+           {K_eq : DecideableEnsembles.Query_eq K}
+           (l : association_list K V)
+           (k : K) (v : V) : list (K * V)  :=
+    (k, v) :: l.
+
+  Instance dns_list_cache : Cache :=
+    {| CacheEncode := option (word 17) * association_list string pointerT;
+       CacheDecode := option (word 17) * association_list pointerT string;
+       Equiv ce cd := fst ce = fst cd
+                      /\ (snd ce) = (map (fun ps => match ps with (p, s) => (s, p) end) (snd cd))
+                      /\ NoDup (map fst (snd cd))
+    |}%type.
+
+  Definition list_CacheEncode_empty : CacheEncode := (Some (wzero _), nil).
+  Definition list_CacheDecode_empty : CacheDecode := (Some (wzero _), nil).
+
+  Lemma list_cache_empty_Equiv : Equiv list_CacheEncode_empty list_CacheDecode_empty.
+  Proof.
+    simpl; intuition; simpl; econstructor.
+  Qed.
+
+  Local Opaque pow2.
+  Arguments natToWord : simpl never.
+  Arguments wordToNat : simpl never.
+
+  (* pointerT2Nat (Nat2pointerT (NPeano.div (wordToNat w) 8)) *)
+
+  Instance cacheAddNat : CacheAdd _ nat :=
+    {| addE ce n := (Ifopt (fst ce) as m Then
+                                         let n' := (wordToNat m) + n in
+                     if Compare_dec.lt_dec n' (pow2 17)
+                     then Some (natToWord _ n')
+                     else None
+                            Else None, snd ce);
+       addD cd n := (Ifopt (fst cd) as m Then
+                                         let n' := (wordToNat m) + n in
+                     if Compare_dec.lt_dec n' (pow2 17)
+                     then Some (natToWord _ n')
+                     else None
+                            Else None, snd cd) |}.
+  Proof.
+    simpl; intuition eauto; destruct a; destruct a0;
+      simpl in *; eauto; try congruence.
+    injections.
+    find_if_inside; eauto.
+  Defined.
+
+  Instance Query_eq_string : Query_eq string :=
+    {| A_eq_dec := string_dec |}.
+
+  Instance : Query_eq pointerT :=
+    {| A_eq_dec := pointerT_eq_dec |}.
+
+  Instance cachePeekDNPointer : CachePeek _ (option pointerT) :=
+    {| peekE ce := Ifopt (fst ce) as m Then Some (Nat2pointerT (wordToNat (wtl (wtl (wtl m))))) Else None;
+       peekD cd := Ifopt (fst cd) as m Then Some
+                                       (Nat2pointerT (wordToNat (wtl (wtl (wtl m)))))
+                                       Else None |}.
+  Proof.
+    abstract (simpl; intros; intuition; rewrite H0; auto).
+  Defined.
+
+  Lemma cacheGetDNPointer_pf
+    : forall (ce : CacheEncode) (cd : CacheDecode)
+             (p : string) (q : pointerT),
+      Equiv ce cd ->
+      (association_list_find_first (snd cd) q = Some p <-> List.In q (association_list_find_all (snd ce) p)).
+  Proof.
+    intros [? ?] [? ?] ? ?; simpl; intuition eauto; subst.
+    - subst; induction a0; simpl in *; try congruence.
+      destruct a; simpl in *; find_if_inside; subst.
+      + inversion H2; subst; intros.
+        find_if_inside; subst; simpl; eauto.
+      + inversion H2; subst; intros.
+        find_if_inside; subst; simpl; eauto; congruence.
+    - subst; induction a0; simpl in *; intuition.
+      destruct a; simpl in *; find_if_inside.
+      + inversion H2; subst; intros.
+        find_if_inside; subst; simpl; eauto; try congruence.
+        apply IHa0 in H1; eauto.
+        elimtype False; apply H3; revert H1; clear.
+        induction a0; simpl; intros; try congruence.
+        destruct a; find_if_inside; injections; auto.
+      + inversion H2; subst; intros.
+        find_if_inside; subst; simpl; eauto; try congruence.
+        simpl in H1; intuition eauto; subst.
+        congruence.
+  Qed.
+
+  Instance cacheGetDNPointer : CacheGet _ string pointerT :=
+    {| getE ce p := association_list_find_all (snd ce) p;
+       getD ce p := association_list_find_first (snd ce) p;
+       get_correct := cacheGetDNPointer_pf |}.
+
+  Lemma cacheAddDNPointer_pf
+    : forall (ce : CacheEncode) (cd : CacheDecode) (t : string * pointerT),
+   Equiv ce cd ->
+   add_ptr_OK t ce cd ->
+   Equiv (fst ce, association_list_add (snd ce) (fst t) (snd t))
+     (fst cd, association_list_add (snd cd) (snd t) (fst t)).
+  Proof.
+    simpl; intuition eauto; simpl in *; subst; eauto.
+    unfold add_ptr_OK in *.
+    destruct t; simpl in *; simpl; econstructor; eauto.
+    clear H3; induction b0; simpl.
+    - intuition.
+    - simpl in H0; destruct a; find_if_inside;
+        try discriminate.
+      intuition.
+  Qed.
+
+  Instance cacheAddDNPointer
+    : CacheAdd_Guarded _ add_ptr_OK :=
+    {| addE_G ce sp := (fst ce, association_list_add (snd ce) (fst sp) (snd sp));
+       addD_G cd sp := (fst cd, association_list_add (snd cd) (snd sp) (fst sp));
+       add_correct_G := cacheAddDNPointer_pf
+    |}.
+
+  Lemma IndependentCaches :
     forall env p (b : nat),
       getD (addD env b) p = getD env p.
-  Variable GetCacheAdd_1 :
-    forall env (p : pointerT) (domain : string),
-      getD (addD env (domain, p)) p = Some domain.
-  Variable GetCacheAdd_2 :
-    forall env (p p' : pointerT) (domain : string),
-      p <> p' -> getD (addD env (domain, p')) p = getD env p.
+  Proof.
+    simpl; intros; eauto.
+  Qed.
+
+  Lemma IndependentCaches' :
+    forall env p (b : nat),
+      getE (addE env b) p = getE env p.
+  Proof.
+    simpl; intros; eauto.
+  Qed.
+
+  Lemma getDistinct :
+    forall env l p p',
+      p <> p'
+      -> getD (addD_G env (l, p)) p' = getD env p'.
+  Proof.
+    simpl; intros; eauto.
+    find_if_inside; try congruence.
+  Qed.
+
+  Lemma getDistinct' :
+    forall env l p p' l',
+      List.In p (getE (addE_G env (l', p')) l)
+      -> p = p' \/ List.In p (getE env l).
+  Proof.
+    simpl in *; intros; intuition eauto.
+    find_if_inside; simpl in *; intuition eauto.
+  Qed.
+
+  Arguments NPeano.div : simpl never.
+
+  Lemma mult_pow2 :
+    forall m n,
+      pow2 m * pow2 n = pow2 (m + n).
+  Proof.
+    Local Transparent pow2.
+    induction m; simpl; intros.
+    - omega.
+    - rewrite <- IHm.
+      rewrite <- !plus_n_O.
+      rewrite Mult.mult_plus_distr_r; omega.
+  Qed.
+
+  Corollary mult_pow2_8 : forall n,
+      8 * (pow2 n) = pow2 (3 + n).
+  Proof.
+    intros; rewrite <- mult_pow2.
+    reflexivity.
+  Qed.
+
+  Local Opaque pow2.
+
+  Lemma pow2_div
+    : forall m n,
+      lt (m + n * 8) (pow2 17)
+      -> lt (NPeano.div m 8) (pow2 14).
+  Proof.
+    intros.
+    eapply (NPeano.Nat.mul_lt_mono_pos_l 8); try omega.
+    rewrite mult_pow2_8.
+    eapply le_lt_trans.
+    apply NPeano.Nat.mul_div_le; try omega.
+    simpl.
+    omega.
+  Qed.
+
+  Lemma addPeekNone :
+    forall env n,
+      peekD env = None
+      -> peekD (addD env n) = None.
+  Proof.
+    simpl; intros.
+    destruct (fst env); simpl in *; congruence.
+  Qed.
+
+  Lemma wtl_div
+    : forall n (w : word (S (S (S n)))),
+      wordToNat (wtl (wtl (wtl w))) = NPeano.div (wordToNat w) 8.
+  Proof.
+    intros.
+    pose proof (shatter_word_S w); destruct_ex; subst.
+    pose proof (shatter_word_S x0); destruct_ex; subst.
+    pose proof (shatter_word_S x2); destruct_ex; subst.
+    simpl wtl.
+    rewrite <- (NPeano.Nat.div_div _ 2 4) by omega.
+    rewrite <- (NPeano.Nat.div_div _ 2 2) by omega.
+    rewrite <- !NPeano.Nat.div2_div.
+    rewrite !div2_WS.
+    reflexivity.
+  Qed.
+
+  Lemma mult_lt_compat_l'
+    : forall (m n p : nat),
+      lt 0 p
+      -> lt (p * n)  (p * m)
+      -> lt n m.
+  Proof.
+    induction m; simpl; intros; try omega.
+    rewrite (mult_comm p 0) in H0; simpl in *; try omega.
+    destruct p; try (elimtype False; auto with arith; omega).
+    inversion H0.
+    rewrite (mult_comm p (S m)) in H0.
+    simpl in H0.
+    destruct n; try omega.
+    rewrite (mult_comm p (S n)) in H0; simpl in H0.
+    apply plus_lt_reg_l in H0.
+    rewrite <- NPeano.Nat.succ_lt_mono.
+    eapply (IHm n p); try eassumption; try omega.
+    rewrite mult_comm.
+    rewrite (mult_comm p m); auto.
+  Qed.
+
+  Lemma mult_lt_compat_l''
+    : forall (p m k n : nat),
+      lt 0 p
+      -> lt n m
+      -> lt k p
+      -> lt ((p * n) + k) (p * m).
+  Proof.
+    induction p; intros; try omega.
+    simpl.
+    inversion H; subst; simpl.
+    inversion H1; subst; omega.
+    destruct k; simpl.
+    - rewrite <- plus_n_O.
+      eapply (mult_lt_compat_l n m (S p)); auto.
+    - assert (lt (p * n + k) (p * m)) by
+          (apply IHp; try omega).
+      omega.
+  Qed.
+
+  Lemma addPeekNone' :
+    forall env n m,
+      peekD env = Some m
+      -> ~ lt (n + (pointerT2Nat m)) (pow2 14)
+      -> peekD (addD env (n * 8)) = None.
+  Proof.
+    simpl; intros; subst.
+    destruct (fst env); simpl in *; try discriminate.
+    injections.
+    find_if_inside; try reflexivity.
+    unfold If_Opt_Then_Else.
+    rewrite !wtl_div in *.
+    elimtype False; apply H0.
+    rewrite pointerT2Nat_Nat2pointerT in *;
+      try (eapply pow2_div; eassumption).
+    eapply (mult_lt_compat_l' _ _ 8); try omega.
+    destruct n; try omega.
+    elimtype False; apply H0.
+    simpl.
+    eapply (mult_lt_compat_l' _ _ 8); try omega.
+    - eapply le_lt_trans.
+      apply NPeano.Nat.mul_div_le; omega.
+      simpl in l.
+      rewrite mult_pow2_8; simpl; omega.
+    - rewrite mult_plus_distr_l.
+      assert (8 <> 0) by omega.
+      pose proof (NPeano.Nat.mul_div_le (wordToNat w) 8 H).
+      apply le_lt_trans with (8 * S n + (wordToNat w)).
+      omega.
+      rewrite mult_pow2_8; simpl; omega.
+  Qed.
+
+  Lemma addPeekSome :
+    forall env n m,
+      peekD env = Some m
+      -> lt (n + (pointerT2Nat m)) (pow2 14)
+      -> exists p',
+          peekD (addD env (n * 8)) = Some p'
+          /\ pointerT2Nat p' = n + (pointerT2Nat m).
+  Proof.
+    simpl; intros; subst.
+    destruct (fst env); simpl in *; try discriminate.
+    injections.
+    find_if_inside.
+    - rewrite !wtl_div in *.
+      rewrite pointerT2Nat_Nat2pointerT in *;
+        try (eapply pow2_div; eassumption).
+      unfold If_Opt_Then_Else.
+      eexists; split; try reflexivity.
+      rewrite wtl_div.
+      rewrite wordToNat_natToWord_idempotent.
+      rewrite pointerT2Nat_Nat2pointerT in *; try omega.
+      rewrite NPeano.Nat.div_add; try omega.
+      rewrite NPeano.Nat.div_add; try omega.
+      apply Nomega.Nlt_in.
+      rewrite Nnat.Nat2N.id, Npow2_nat; auto.
+    - elimtype False; apply n0.
+      rewrite !wtl_div in *.
+      rewrite pointerT2Nat_Nat2pointerT in *.
+      rewrite (NPeano.div_mod (wordToNat w) 8); try omega.
+      pose proof (mult_pow2_8 14) as H'; simpl plus in H'; rewrite <- H'.
+      replace (8 * NPeano.div (wordToNat w) 8 + NPeano.modulo (wordToNat w) 8 + n * 8)
+      with (8 * (NPeano.div (wordToNat w) 8 + n) + NPeano.modulo (wordToNat w) 8)
+        by omega.
+      eapply mult_lt_compat_l''; try omega.
+      apply NPeano.Nat.mod_upper_bound; omega.
+      eapply (mult_lt_compat_l' _ _ 8); try omega.
+      eapply le_lt_trans.
+      apply NPeano.Nat.mul_div_le; omega.
+      rewrite mult_pow2_8; simpl.
+      apply wordToNat_bound.
+  Qed.
+
+  Lemma addZeroPeek :
+    forall xenv,
+      peekD xenv = peekD (addD xenv 0).
+  Proof.
+    simpl; intros.
+    destruct (fst xenv); simpl; eauto.
+    find_if_inside; unfold If_Opt_Then_Else.
+    rewrite <- plus_n_O, natToWord_wordToNat; auto.
+    elimtype False; apply n.
+    rewrite <- plus_n_O.
+    apply wordToNat_bound.
+  Qed.
+
+  Local Opaque wordToNat.
+  Local Opaque natToWord.
+
+  Lemma boundPeekSome :
+    forall env n m m',
+      peekD env = Some m
+      -> peekD (addD env (n * 8)) = Some m'
+      -> lt (n + (pointerT2Nat m)) (pow2 14).
+  Proof.
+    simpl; intros; subst.
+    destruct (fst env); simpl in *; try discriminate.
+    injections.
+    find_if_inside; unfold If_Opt_Then_Else in *; try congruence.
+    injections.
+    rewrite !wtl_div in *.
+    rewrite pointerT2Nat_Nat2pointerT in *;
+      try (eapply pow2_div; eassumption).
+    eapply (mult_lt_compat_l' _ _ 8); try omega.
+    - rewrite mult_plus_distr_l.
+      assert (8 <> 0) by omega.
+      pose proof (NPeano.Nat.mul_div_le (wordToNat w) 8 H).
+      apply le_lt_trans with (8 * n + (wordToNat w)).
+      omega.
+      rewrite mult_pow2_8.
+      simpl plus at -1.
+      omega.
+  Qed.
+
+  Lemma addPeekESome :
+    forall env n m,
+      peekE env = Some m
+      -> lt (n + (pointerT2Nat m)) (pow2 14)%nat
+      -> exists p',
+          peekE (addE env (n * 8)) = Some p'
+          /\ pointerT2Nat p' = n + (pointerT2Nat m).
+  Proof.
+        simpl; intros; subst.
+    destruct (fst env); simpl in *; try discriminate.
+    injections.
+    find_if_inside.
+    - rewrite !wtl_div in *.
+      rewrite pointerT2Nat_Nat2pointerT in *;
+        try (eapply pow2_div; eassumption).
+      unfold If_Opt_Then_Else.
+      eexists; split; try reflexivity.
+      rewrite wtl_div.
+      rewrite wordToNat_natToWord_idempotent.
+      rewrite pointerT2Nat_Nat2pointerT in *; try omega.
+      rewrite NPeano.Nat.div_add; try omega.
+      rewrite NPeano.Nat.div_add; try omega.
+      apply Nomega.Nlt_in.
+      rewrite Nnat.Nat2N.id, Npow2_nat; auto.
+    - elimtype False; apply n0.
+      rewrite !wtl_div in *.
+      rewrite pointerT2Nat_Nat2pointerT in *.
+      rewrite (NPeano.div_mod (wordToNat w) 8); try omega.
+      pose proof (mult_pow2_8 14) as H'; simpl plus in H'; rewrite <- H'.
+      replace (8 * NPeano.div (wordToNat w) 8 + NPeano.modulo (wordToNat w) 8 + n * 8)
+      with (8 * (NPeano.div (wordToNat w) 8 + n) + NPeano.modulo (wordToNat w) 8)
+        by omega.
+      eapply mult_lt_compat_l''; try omega.
+      apply NPeano.Nat.mod_upper_bound; omega.
+      eapply (mult_lt_compat_l' _ _ 8); try omega.
+      eapply le_lt_trans.
+      apply NPeano.Nat.mul_div_le; omega.
+      rewrite mult_pow2_8; simpl.
+      apply wordToNat_bound.
+  Qed.
+
+  Lemma boundPeekESome :
+    forall env n m m',
+      peekE env = Some m
+      -> peekE (addE env (n * 8)) = Some m'
+      -> lt (n + (pointerT2Nat m)) (pow2 14).
+  Proof.
+    simpl; intros; subst.
+    destruct (fst env); simpl in *; try discriminate.
+    injections.
+    find_if_inside; unfold If_Opt_Then_Else in *; try congruence.
+    injections.
+    rewrite !wtl_div in *.
+    rewrite pointerT2Nat_Nat2pointerT in *;
+      try (eapply pow2_div; eassumption).
+    eapply (mult_lt_compat_l' _ _ 8); try omega.
+    - rewrite mult_plus_distr_l.
+      assert (8 <> 0) by omega.
+      pose proof (NPeano.Nat.mul_div_le (wordToNat w) 8 H).
+      apply le_lt_trans with (8 * n + (wordToNat w)).
+      omega.
+      rewrite mult_pow2_8.
+      simpl plus at -1.
+      omega.
+  Qed.
+
+  Lemma addPeekENone :
+      forall env n,
+        peekE env = None
+        -> peekE (addE env n) = None.
+  Proof.
+    simpl; intros.
+    destruct (fst env); simpl in *; congruence.
+  Qed.
+
+  Lemma addPeekENone' :
+    forall env n m,
+      peekE env = Some m
+      -> ~ lt (n + (pointerT2Nat m)) (pow2 14)%nat
+      -> peekE (addE env (n * 8)) = None.
+  Proof.
+    simpl; intros; subst.
+    destruct (fst env); simpl in *; try discriminate.
+    injections.
+    find_if_inside; try reflexivity.
+    unfold If_Opt_Then_Else.
+    rewrite !wtl_div in *.
+    elimtype False; apply H0.
+    rewrite pointerT2Nat_Nat2pointerT in *;
+      try (eapply pow2_div; eassumption).
+    eapply (mult_lt_compat_l' _ _ 8); try omega.
+    destruct n; try omega.
+    elimtype False; apply H0.
+    simpl.
+    eapply (mult_lt_compat_l' _ _ 8); try omega.
+    - eapply le_lt_trans.
+      apply NPeano.Nat.mul_div_le; omega.
+      simpl in l.
+      rewrite mult_pow2_8; simpl; omega.
+    - rewrite mult_plus_distr_l.
+      assert (8 <> 0) by omega.
+      pose proof (NPeano.Nat.mul_div_le (wordToNat w) 8 H).
+      apply le_lt_trans with (8 * S n + (wordToNat w)).
+      omega.
+      rewrite mult_pow2_8; simpl; omega.
+  Qed.
+
+  Lemma addZeroPeekE :
+    forall xenv,
+      peekE xenv = peekE (addE xenv 0).
+  Proof.
+    simpl; intros.
+    destruct (fst xenv); simpl; eauto.
+    find_if_inside; unfold If_Opt_Then_Else.
+    rewrite <- plus_n_O, natToWord_wordToNat; auto.
+    elimtype False; apply n.
+    rewrite <- plus_n_O.
+    apply wordToNat_bound.
+  Qed.
+
+  Import Vectors.VectorDef.VectorNotations.
 
   Definition GoodCache (env : CacheDecode) :=
     forall domain p,
@@ -145,49 +640,42 @@ Section DnsPacket.
     : forall cd p p0 domain domain',
       GoodCache cd
       -> ValidDomainName domain' /\ (String.length domain' > 0)%nat
-      -> getD (addD cd (domain', p0)) p = Some domain
+      -> getD (addD_G cd (domain', p0)) p = Some domain
       -> forall pre label post : string,
           domain = (pre ++ label ++ post)%string ->
           ValidLabel label -> (String.length label <= 63)%nat.
   Proof.
-    unfold GoodCache; intros.
-    destruct (ptr_eq_dec p p0); subst.
-    - rewrite GetCacheAdd_1 in H1; injections.
-      destruct H0.
-      eapply H0; eauto.
-    - rewrite GetCacheAdd_2 in H1 by eauto.
-      eapply H; eauto.
+    unfold GoodCache; simpl; intros.
+    destruct (pointerT_eq_dec p p0); subst.
+    - injections; intuition.
+      eapply H1; eauto.
+    - eapply H; eauto.
   Qed.
 
   Lemma cacheIndependent_add_9
     : forall cd p p0 domain domain',
       GoodCache cd
       -> ValidDomainName domain' /\ (String.length domain' > 0)%nat
-      -> getD (addD cd (domain', p0)) p = Some domain
+      -> getD (addD_G cd (domain', p0)) p = Some domain
       -> ValidDomainName domain.
   Proof.
-    unfold GoodCache; intros.
-    destruct (ptr_eq_dec p p0); subst.
-    - rewrite GetCacheAdd_1 in H1; injections.
-      destruct H0.
-      eapply H0; eauto.
-    - rewrite GetCacheAdd_2 in H1 by eauto.
-      eapply H; eauto.
+    unfold GoodCache; simpl; intros.
+    destruct (pointerT_eq_dec p p0); subst.
+    - injections; intuition.
+    - eapply H; eauto.
   Qed.
 
   Lemma cacheIndependent_add_10
     : forall cd p p0 domain domain',
       GoodCache cd
       -> ValidDomainName domain' /\ (String.length domain' > 0)%nat
-      -> getD (addD cd (domain', p0)) p = Some domain
+      -> getD (addD_G cd (domain', p0)) p = Some domain
       -> gt (String.length domain) 0.
   Proof.
-    unfold GoodCache; intros.
-    destruct (ptr_eq_dec p p0); subst.
-    - rewrite GetCacheAdd_1 in H1; injections.
-      destruct H0; apply H1.
-    - rewrite GetCacheAdd_2 in H1 by eauto.
-      eapply H; eauto.
+    unfold GoodCache; simpl; intros.
+    destruct (pointerT_eq_dec p p0); subst.
+    - injections; intuition.
+    - eapply H; eauto.
   Qed.
 
   Ltac solve_GoodCache_inv foo :=
